ulib/FStar.Reader.fst
@@ -1,82 +1,43 @@
 module FStar.Reader
-let reader_pre_h  (heap:Type)          = heap -> GTot Type0
-let reader_post_h (a:Type)             = a -> GTot Type0
-let reader_wp_h   (heap:Type) (a:Type) = reader_post_h a -> Tot (reader_pre_h heap)
 
-unfold let reader_return        (heap:Type) (a:Type)
-                               (x:a) (p:reader_post_h a) (h0:heap) = p x
-unfold let reader_bind_wp   (heap:Type) 
-			    (r1:range) 
-			    (a:Type) (b:Type)
-                            (wp1:reader_wp_h heap a)
-                            (wp2:(a -> GTot (reader_wp_h heap b)))
-                            (p:reader_post_h b) (h0:heap) =
-     labeled r1 "push" unit
-     /\ wp1 (fun a ->
-       labeled r1 "pop" unit
-       /\ wp2 a p h0) h0
-unfold let reader_if_then_else  (heap:Type) (a:Type) (p:Type)
-                             (wp_then:reader_wp_h heap a) (wp_else:reader_wp_h heap a)
-                             (post:reader_post_h a) (h0:heap) =
-     l_ITE p
-        (wp_then post h0)
-	(wp_else post h0)
-unfold let reader_ite_wp        (heap:Type) (a:Type)
-                            (wp:reader_wp_h heap a)
-                            (post:reader_post_h a) (h0:heap) =
-     forall (k:reader_post_h a).
-	 (forall (x:a).{:pattern (guard_free (k x))} k x <==> post x)
-	 ==> wp k h0
-unfold let reader_stronger  (heap:Type) (a:Type) (wp1:reader_wp_h heap a)
-                        (wp2:reader_wp_h heap a) =
-     (forall (p:reader_post_h a) (h:heap). wp1 p h ==> wp2 p h)
+type reader (heap:Type) (a:Type) = heap -> M a
 
-unfold let reader_close_wp      (heap:Type) (a:Type) (b:Type)
-                             (wp:(b -> GTot (reader_wp_h heap a)))
-                             (p:reader_post_h a) (h:heap) =
-     (forall (b:b). wp b p h)
-unfold let reader_assert_p      (heap:Type) (a:Type) (p:Type)
-                             (wp:reader_wp_h heap a)
-                             (q:reader_post_h a) (h:heap) =
-     p /\ wp q h
-unfold let reader_assume_p      (heap:Type) (a:Type) (p:Type)
-                             (wp:reader_wp_h heap a)
-                             (q:reader_post_h a) (h:heap) =
-     p ==> wp q h
-unfold let reader_null_wp       (heap:Type) (a:Type)
-                             (p:reader_post_h a) (h:heap) =
-     (forall (x:a). p x)
-unfold let reader_trivial       (heap:Type) (a:Type)
-                             (wp:reader_wp_h heap a) =
-     (forall h0. wp (fun r -> True) h0)
+let return_reader (heap:Type) (a:Type) (x:a) : reader heap a = fun h -> x
+let bind_reader (heap:Type) (a:Type) (b:Type) (x:reader heap a) (f:a -> reader heap b) : reader heap b =
+  fun h0 -> let x0 = x h0 in f x0 h0
+   (* TODO : elaboration should also work with *)
+   (* fun h0 -> f (x0 h0) h0 *)
+let get_reader (heap:Type) () : reader heap heap = fun h -> h
 
-new_effect {
-  READER_h (heap:Type) : result:Type -> wp:reader_wp_h heap result -> Effect
-  with return_wp    = reader_return heap
-     ; bind_wp      = reader_bind_wp heap
-     ; if_then_else = reader_if_then_else heap
-     ; ite_wp       = reader_ite_wp heap
-     ; stronger     = reader_stronger heap
-     ; close_wp     = reader_close_wp heap
-     ; assert_p     = reader_assert_p heap
-     ; assume_p     = reader_assume_p heap
-     ; null_wp      = reader_null_wp heap
-     ; trivial      = reader_trivial heap
+new_effect_for_free {
+  READER_h (heap:Type) : a:Type -> Effect
+  with repr  = reader heap
+    ; bind   = bind_reader heap
+    ; return = return_reader heap
+  and effect_actions
+    get = get_reader heap
 }
+
+let reader_pre_h  = READER_h.pre
+let reader_post_h = READER_h.post
+let reader_wp_h   = READER_h.wp
+
 open FStar.Heap
-new_effect READER = READER_h FStar.Heap.heap
+
+new_effect_for_free READER = READER_h FStar.Heap.heap
 
 effect STRead (a:Type) (pre: (heap -> Type0)) (post:heap -> a -> Type0) = 
-  READER a (fun (p:reader_post_h a) h0 -> pre h0 /\ (forall (x:a). post h0 x ==> p x))
+  READER a (fun h0 (p:reader_post_h FStar.Heap.heap a) -> pre h0 /\ (forall (x:a). post h0 x ==> p x))
 
 open FStar.ST
+
 assume val read:  #a:Type -> r:ref a -> STRead a
 					 (requires (fun h -> True))
 					 (ensures (fun h x -> x == sel h r))
 
-unfold let lift_reader_state (a:Type) (wp:reader_wp_h heap a) (p:st_post a) (h:heap) = wp (fun a -> p a h) h
+unfold let lift_reader_state (a:Type) (wp:reader_wp_h heap a) (h:heap) (p:st_post a) = wp h (fun a -> p (a, h))
 sub_effect READER ~> STATE = lift_reader_state
-unfold let lift_div_reader (a:Type) (wp:pure_wp a) (p:reader_post_h a) (h:heap) = wp p
+unfold let lift_div_reader (a:Type) (wp:pure_wp a) (h:heap) (p:reader_post_h FStar.Heap.heap a) = wp p
 sub_effect DIV ~> READER = lift_div_reader
 
 (* Testing *)
@@ -89,7 +50,7 @@ let f (r:ref int) : STRead int
 
 let g (r:ref int) (s:ref int) : ST unit
   (requires (fun h -> True))
-  (ensures (fun h0 _ h1 -> sel h1 r = (sel h0 r + 1) + (sel h0 s + 1)))
+  (ensures (fun h0 (_, h1) -> sel h1 r = (sel h0 r + 1) + (sel h0 s + 1)))
   = let x = f r in
     let y = f s in
     r := x + y
